theories/std/chunk.v
@@ -1,5 +1,5 @@
 From ml Require Import
-  prelude.
+prelude.
 From ml.bi Require Import
   big_op.
 From ml.language Require Import
@@ -20,17 +20,17 @@ Section heapGS.
     λ: "sz" "v",
       if: #0 < "sz" then (
         AllocN "sz" "v"
-) else (
+      ) else (
         #(inhabitant : loc)
       ).
 
   #[local] Definition chunk_foldli_aux : val :=
     rec: "chunk_foldli_aux" "t" "sz" "acc" "fn" "i" :=
-      if: "i" = "sz" then (
-        "acc"
+      if: "sz" ≤ "i" then (
+"acc"
       ) else (
         "chunk_foldli_aux" "t" "sz" ("fn" "acc" "i" !("t" +ₗ "i")) "fn" (#1 + "i")
-).
+      ).
   Definition chunk_foldli : val :=
     λ: "t" "sz" "acc" "fn",
       chunk_foldli_aux "t" "sz" "acc" "fn" #0.
@@ -40,7 +40,7 @@ Section heapGS.
 
   #[local] Definition chunk_foldri_aux : val :=
     rec: "chunk_foldri_aux" "t" "fn" "acc" "i" :=
-      if: "i" = #0 then (
+      if: "i" ≤ #0 then (
         "acc"
       ) else (
         let: "i" := "i" - #1 in
@@ -573,7 +573,6 @@ Section heapGS.
   )%I.
 
   Lemma chunk_make_spec sz v :
-    (0 ≤ sz)%Z →
     {{{ True }}}
       chunk_make #sz v
     {{{ l,
@@ -582,14 +581,16 @@ Section heapGS.
       if decide (0 < sz)%Z then meta_token l ⊤ else True
     }}}.
   Proof.
-    iIntros "% %Φ _ HΦ".
+    iIntros "%Φ _ HΦ".
     wp_rec. wp_pures.
     case_bool_decide; wp_pures.
     - setoid_rewrite decide_True; [| done..].
       wp_apply (wp_allocN with "[//]"); first done. iIntros "%l (H↦ & Hmeta)".
       destruct (Z.to_nat sz) eqn:Heq; first lia. iDestruct "Hmeta" as "(Hmeta & _)". rewrite Loc.add_0.
       iApply "HΦ". rewrite /array. iFrame.
-    - assert (sz = 0) as -> by lia. iSmash.
+    - iApply "HΦ".
+      rewrite Z2Nat.nonpos; last lia. rewrite decide_False; last lia. rewrite right_id.
+      iApply chunk_model_nil.
   Qed.
 
   Lemma chunk_get_spec v l (i : Z) dq vs E :
@@ -604,7 +605,7 @@ Section heapGS.
       chunk_model l dq vs
     }}}.
   Proof.
-    iIntros "% % %Φ Hmodel HΦ".
+    iIntros "%Hi %Hlookup %Φ Hmodel HΦ".
     iDestruct (chunk_model_lookup_acc with "Hmodel") as "(H↦ & Hmodel)"; first done.
     rewrite (Z2Nat.id i) //. wp_load.
     iSmash.
@@ -621,7 +622,7 @@ Section heapGS.
       chunk_model l (DfracOwn 1) (<[Z.to_nat i := v]> vs)
     }}}.
   Proof.
-    iIntros "% %Φ Hmodel HΦ".
+    iIntros "%Hi %Φ Hmodel HΦ".
     iDestruct (chunk_model_update with "Hmodel") as "(H↦ & Hmodel)".
     { destruct (nth_lookup_or_length vs (Z.to_nat i) inhabitant); [done | lia]. }
     rewrite (Z2Nat.id i); last lia. wp_store.
@@ -629,15 +630,15 @@ Section heapGS.
   Qed.
 
   #[local] Lemma chunk_foldli_aux_spec i vs Ψ l (sz : Z) acc fn :
-    (i ≤ sz)%Z →
+    i ≤ Z.to_nat sz →
     i = length vs →
     {{{
-      Ψ i vs None acc ∗
+      ▷ Ψ i vs None acc ∗
       □ (
         ∀ i vs acc,
         ⌜i < Z.to_nat sz ∧ i = length vs⌝ -∗
         Ψ i vs None acc -∗
-        chunk_au_load l i (λ v,
+        chunk_au_load l i (λ v, ▷
           Ψ i vs (Some v) acc
         )
       ) ∗
@@ -645,7 +646,7 @@ Section heapGS.
         ∀ i vs v acc,
         ⌜i < Z.to_nat sz ∧ i = length vs⌝ -∗
         Ψ i vs (Some v) acc -∗
-        WP fn acc #i v {{ acc,
+        WP fn acc #i v {{ acc, ▷
           Ψ (S i) (vs ++ [v]) None acc
         }}
       )
@@ -658,17 +659,18 @@ Section heapGS.
     }}}.
   Proof.
     iIntros "%Hi1 %Hi2 %Φ (HΨ & #Hau & #Hfn) HΦ".
-    Z_to_nat sz. rewrite Nat2Z.id. remember (sz - i) as j eqn:Hj.
+    remember (Z.to_nat sz - i) as j eqn:Hj.
     iInduction j as [| j] "IH" forall (i vs acc Hi1 Hi2 Hj);
-      wp_rec; wp_pures.
+      wp_rec; wp_pure credit:"H£"; wp_pures.
     - rewrite bool_decide_eq_true_2; last (repeat f_equal; lia). wp_pures.
       iApply ("HΦ" $! []).
-      rewrite !right_id. assert (sz = i) by lia. iSmash.
+      rewrite !right_id. assert (Z.to_nat sz = i) as -> by lia. iSmash.
     - rewrite bool_decide_eq_false_2; last naive_solver lia. wp_pures.
       wp_bind (!_)%E.
       iMod ("Hau" $! i with "[] HΨ") as "(%dq & %v & H↦ & _ & HΨ)"; first iSmash.
       wp_load.
       iMod ("HΨ" with "H↦") as "HΨ". iModIntro.
+      iMod (lc_fupd_elim_later with "H£ HΨ") as "HΨ".
       wp_apply (wp_wand with "(Hfn [] HΨ)"); first iSmash. iIntros "%acc' HΨ".
       rewrite Z.add_1_l -Nat2Z.inj_succ.
       wp_apply ("IH" with "[] [] [] HΨ [HΦ]"); rewrite ?app_length; [iSmash.. |].
@@ -677,14 +679,13 @@ Section heapGS.
       rewrite -(assoc (++)). iSmash.
   Qed.
   Lemma chunk_foldli_spec_atomic Ψ l sz acc fn :
-    (0 ≤ sz)%Z →
     {{{
-      Ψ 0 [] None acc ∗
+      ▷ Ψ 0 [] None acc ∗
       □ (
         ∀ i vs acc,
         ⌜i < Z.to_nat sz ∧ i = length vs⌝ -∗
         Ψ i vs None acc -∗
-        chunk_au_load l i (λ v,
+        chunk_au_load l i (λ v, ▷
           Ψ i vs (Some v) acc
         )
       ) ∗
@@ -692,7 +693,7 @@ Section heapGS.
         ∀ i vs v acc,
         ⌜i < Z.to_nat sz ∧ i = length vs⌝ -∗
         Ψ i vs (Some v) acc -∗
-        WP fn acc #i v {{ acc,
+        WP fn acc #i v {{ acc, ▷
           Ψ (S i) (vs ++ [v]) None acc
         }}
       )
@@ -704,21 +705,21 @@ Section heapGS.
       Ψ (Z.to_nat sz) vs None acc
     }}}.
   Proof.
-    iIntros "%Hsz %Φ (HΨ & #Hau & #Hfn) HΦ".
+    iIntros "%Φ (HΨ & #Hau & #Hfn) HΦ".
     wp_rec.
-    wp_smart_apply (chunk_foldli_aux_spec 0 [] Ψ with "[$HΨ] HΦ"); [done.. |].
+    wp_smart_apply (chunk_foldli_aux_spec 0 [] Ψ with "[$HΨ] HΦ"); [lia | done |].
     auto with iFrame.
   Qed.
   Lemma chunk_foldli_spec Ψ l dq vs (sz : Z) acc fn :
-    sz = length vs →
+    Z.to_nat sz = length vs →
     {{{
       chunk_model l dq vs ∗
-      Ψ 0 [] acc ∗
+      ▷ Ψ 0 [] acc ∗
       □ (
         ∀ i v acc,
         ⌜vs !! i = Some v⌝ -∗
         Ψ i (take i vs) acc -∗
-        WP fn acc #i v {{ acc,
+        WP fn acc #i v {{ acc, ▷
           Ψ (S i) (take i vs ++ [v]) acc
         }}
       )
@@ -751,17 +752,16 @@ Section heapGS.
       feed pose proof (list_lookup_lookup_total_lt vs i); first lia.
       wp_apply (wp_wand with "(Hfn [] HΨ)"); first iSmash. clear acc. iIntros "%acc HΨ". iFrame.
       erewrite take_S_r; done.
-    - lia.
   Qed.
   Lemma chunk_foldli_spec' Ψ l dq vs (sz : Z) acc fn :
-    sz = length vs →
+    Z.to_nat sz = length vs →
     {{{
       chunk_model l dq vs ∗
-      Ψ 0 [] acc ∗
+      ▷ Ψ 0 [] acc ∗
       ( [∗ list] i ↦ v ∈ vs,
         ∀ acc,
         Ψ i (take i vs) acc -∗
-        WP fn acc #i v {{ acc,
+        WP fn acc #i v {{ acc, ▷
           Ψ (S i) (take i vs ++ [v]) acc
         }}
       )
@@ -789,14 +789,13 @@ Section heapGS.
   Qed.
 
   Lemma chunk_foldl_spec_atomic Ψ l sz acc fn :
-    (0 ≤ sz)%Z →
     {{{
-      Ψ 0 [] None acc ∗
+      ▷ Ψ 0 [] None acc ∗
       □ (
         ∀ i vs acc,
         ⌜i < Z.to_nat sz ∧ i = length vs⌝ -∗
         Ψ i vs None acc -∗
-        chunk_au_load l i (λ v,
+        chunk_au_load l i (λ v, ▷
           Ψ i vs (Some v) acc
         )
       ) ∗
@@ -804,7 +803,7 @@ Section heapGS.
         ∀ i vs v acc,
         ⌜i < Z.to_nat sz ∧ i = length vs⌝ -∗
         Ψ i vs (Some v) acc -∗
-        WP fn acc v {{ acc,
+        WP fn acc v {{ acc, ▷
           Ψ (S i) (vs ++ [v]) None acc
         }}
       )
@@ -816,21 +815,21 @@ Section heapGS.
       Ψ (Z.to_nat sz) vs None acc
     }}}.
   Proof.
-    iIntros "%Hsz %Φ (HΨ & #Hau & #Hfn) HΦ".
+    iIntros "%Φ (HΨ & #Hau & #Hfn) HΦ".
     wp_rec.
-    wp_smart_apply (chunk_foldli_spec_atomic Ψ with "[$HΨ $Hau] HΦ"); first done.
+    wp_smart_apply (chunk_foldli_spec_atomic Ψ with "[$HΨ $Hau] HΦ").
     iSmash.
   Qed.
   Lemma chunk_foldl_spec Ψ l dq vs (sz : Z) acc fn :
-    sz = length vs →
+    Z.to_nat sz = length vs →
     {{{
       chunk_model l dq vs ∗
-      Ψ 0 [] acc ∗
+      ▷ Ψ 0 [] acc ∗
       □ (
         ∀ i v acc,
         ⌜vs !! i = Some v⌝ -∗
         Ψ i (take i vs) acc -∗
-        WP fn acc v {{ acc,
+        WP fn acc v {{ acc, ▷
           Ψ (S i) (take i vs ++ [v]) acc
         }}
       )
@@ -848,14 +847,14 @@ Section heapGS.
     iSmash.
   Qed.
   Lemma chunk_foldl_spec' Ψ l dq vs (sz : Z) acc fn :
-    sz = length vs →
+    Z.to_nat sz = length vs →
     {{{
       chunk_model l dq vs ∗
-      Ψ 0 [] acc ∗
+      ▷ Ψ 0 [] acc ∗
       ( [∗ list] i ↦ v ∈ vs,
         ∀ acc,
         Ψ i (take i vs) acc -∗
-        WP fn acc v {{ acc,
+        WP fn acc v {{ acc, ▷
           Ψ (S i) (take i vs ++ [v]) acc
         }}
       )
@@ -874,23 +873,23 @@ Section heapGS.
     iSmash.
   Qed.
 
-  #[local] Lemma chunk_foldri_aux_spec sz i vs Ψ l fn acc :
-    i + length vs = sz →
+  #[local] Lemma chunk_foldri_aux_spec (sz i : Z) vs Ψ l fn acc :
+    Z.to_nat i + length vs = Z.to_nat sz →
     {{{
-      Ψ i acc None vs ∗
+      ▷ Ψ (Z.to_nat i) acc None vs ∗
       □ (
         ∀ i acc vs,
-        ⌜(S i + length vs)%nat = sz⌝ -∗
+        ⌜(S i + length vs)%nat = Z.to_nat sz⌝ -∗
         Ψ (S i) acc None vs -∗
-        chunk_au_load l i (λ v,
+        chunk_au_load l i (λ v, ▷
           Ψ (S i) acc (Some v) vs
         )
       ) ∗
       □ (
         ∀ i v acc vs,
-        ⌜(S i + length vs)%nat = sz⌝ -∗
+        ⌜(S i + length vs)%nat = Z.to_nat sz⌝ -∗
         Ψ (S i) acc (Some v) vs -∗
-        WP fn #i v acc {{ acc,
+        WP fn #i v acc {{ acc, ▷
           Ψ i acc None (v :: vs)
         }}
       )
@@ -898,33 +897,37 @@ Section heapGS.
       chunk_foldri_aux #l fn acc #i
     {{{ acc vs',
       RET acc;
-      ⌜(length vs' + length vs)%nat = sz⌝ ∗
+      ⌜(length vs' + length vs)%nat = Z.to_nat sz⌝ ∗
       Ψ 0 acc None (vs' ++ vs)
     }}}.
   Proof.
     iIntros "%Hi %Φ (HΨ & #Hau & #Hfn) HΦ".
-    iInduction i as [| i] "IH" forall (vs acc Hi);
-      wp_rec; wp_pures.
-    - iApply ("HΦ" $! _ []).
+    remember (Z.to_nat i) as j eqn:Hj.
+    iInduction j as [| j] "IH" forall (i vs acc Hi Hj);
+      wp_rec; wp_pure credit:"H£"; wp_pures.
+    - rewrite bool_decide_eq_true_2; last lia. wp_pures.
+      iApply ("HΦ" $! _ []).
       iSmash.
-    - wp_bind (!_)%E.
-      iMod ("Hau" $! i with "[] HΨ") as "(%dq & %v & H↦ & _ & HΨ)"; first iSmash.
-      rewrite Z.sub_1_r -Nat2Z.inj_pred /=; last lia. wp_load.
+    - rewrite bool_decide_eq_false_2; last lia. wp_pures.
+      assert (i = S j) as -> by lia. rewrite Z.sub_1_r -Nat2Z.inj_pred /=; last lia.
+      wp_bind (!_)%E.
+      iMod ("Hau" $! j with "[] HΨ") as "(%dq & %v & H↦ & _ & HΨ)"; first iSmash.
+      wp_load.
       iMod ("HΨ" with "H↦") as "HΨ". iModIntro.
+      iMod (lc_fupd_elim_later with "H£ HΨ") as "HΨ".
       wp_apply (wp_wand with "(Hfn [] HΨ)"); first iSmash. iIntros "%acc' HΨ".
-      wp_apply ("IH" with "[] HΨ [HΦ]"); rewrite ?app_length; [iSmash.. |]. clear acc. iIntros "!> %acc %vs' (<- & HΨ)".
+      wp_apply ("IH" with "[] [] HΨ [HΦ]"); rewrite ?app_length; [iSmash.. |]. clear acc. iIntros "!> %acc %vs' (<- & HΨ)".
       iApply ("HΦ" $! _ (vs' ++ [v])).
       rewrite app_length -(assoc (++)). iSmash.
   Qed.
   Lemma chunk_foldri_spec_atomic Ψ l sz fn acc :
-    (0 ≤ sz)%Z →
     {{{
-      Ψ (Z.to_nat sz) acc None [] ∗
+      ▷ Ψ (Z.to_nat sz) acc None [] ∗
       □ (
         ∀ i acc vs,
         ⌜(S i + length vs)%nat = Z.to_nat sz⌝ -∗
         Ψ (S i) acc None vs -∗
-        chunk_au_load l i (λ v,
+        chunk_au_load l i (λ v, ▷
           Ψ (S i) acc (Some v) vs
         )
       ) ∗
@@ -932,7 +935,7 @@ Section heapGS.
         ∀ i v acc vs,
         ⌜(S i + length vs)%nat = Z.to_nat sz⌝ -∗
         Ψ (S i) acc (Some v) vs -∗
-        WP fn #i v acc {{ acc,
+        WP fn #i v acc {{ acc, ▷
           Ψ i acc None (v :: vs)
         }}
       )
@@ -944,22 +947,23 @@ Section heapGS.
       Ψ 0 acc None vs
     }}}.
   Proof.
-    iIntros "%Hsz %Φ (HΨ & #Hau & #Hfn) HΦ".
-    Z_to_nat sz. rewrite Nat2Z.id.
+    iIntros "%Φ (HΨ & #Hau & #Hfn) HΦ".
     wp_rec.
-    wp_smart_apply (chunk_foldri_aux_spec sz sz [] Ψ with "[$HΨ $Hau $Hfn] [HΦ]"); first done. clear acc. iIntros "!> %acc %vs".
+    wp_smart_apply (chunk_foldri_aux_spec sz sz [] Ψ with "[$HΨ $Hau $Hfn] [HΦ]").
+    { rewrite right_id. lia. }
+    clear acc. iIntros "!> %acc %vs".
     rewrite !right_id. iSmash.
   Qed.
   Lemma chunk_foldri_spec Ψ l dq vs (sz : Z) fn acc :
-    sz = length vs →
+    Z.to_nat sz = length vs →
     {{{
       chunk_model l dq vs ∗
-      Ψ (Z.to_nat sz) acc [] ∗
+      ▷ Ψ (Z.to_nat sz) acc [] ∗
       □ (
         ∀ i v acc,
         ⌜vs !! i = Some v⌝ -∗
         Ψ (S i) acc (drop (S i) vs) -∗
-        WP fn #i v acc {{ acc,
+        WP fn #i v acc {{ acc, ▷
           Ψ i acc (v :: drop (S i) vs)
         }}
       )
@@ -971,17 +975,16 @@ Section heapGS.
       Ψ 0 acc vs
     }}}.
   Proof.
-    iIntros (->) "%Φ (Hmodel & HΨ & #Hfn) HΦ".
+    iIntros "%Hsz %Φ (Hmodel & HΨ & #Hfn) HΦ".
     pose (Ψ' i acc o vs_done := (
       ⌜vs_done = drop i vs⌝ ∗
       chunk_model l dq vs ∗
       Ψ i acc vs_done ∗
       ⌜from_option (λ v, v = vs !!! (i - 1)) True o⌝%I
     )%I).
-    wp_apply (chunk_foldri_spec_atomic Ψ' with "[$Hmodel $HΨ]"); [lia | | iSmash].
-    rewrite Nat2Z.id.
+    wp_apply (chunk_foldri_spec_atomic Ψ' with "[$Hmodel $HΨ]"); last iSmash.
     repeat iSplitR.
-    - rewrite drop_all. iSmash.
+    - rewrite Hsz drop_all. iSmash.
     - clear acc. iIntros "!> %i %acc %vs_done %Hi (-> & Hmodel & HΨ & _)".
       feed pose proof (list_lookup_lookup_total_lt vs i); first lia.
       iDestruct (chunk_model_lookup_acc with "Hmodel") as "(H↦ & Hmodel)"; first done.
@@ -995,14 +998,14 @@ Section heapGS.
       iPureIntro. rewrite -drop_S ?Hlookup; repeat f_equal; lia.
   Qed.
   Lemma chunk_foldri_spec' Ψ l dq vs (sz : Z) fn acc :
-    sz = length vs →
+    Z.to_nat sz = length vs →
     {{{
       chunk_model l dq vs ∗
-      Ψ (Z.to_nat sz) acc [] ∗
+      ▷ Ψ (Z.to_nat sz) acc [] ∗
       ( [∗ list] i ↦ v ∈ vs,
         ∀ acc,
         Ψ (S i) acc (drop (S i) vs) -∗
-        WP fn #i v acc {{ acc,
+        WP fn #i v acc {{ acc, ▷
           Ψ i acc (v :: drop (S i) vs)
         }}
       )
@@ -1014,7 +1017,7 @@ Section heapGS.
       Ψ 0 acc vs
     }}}.
   Proof.
-    iIntros (->) "%Φ (Hmodel & HΨ & Hfn) HΦ".
+    iIntros "%Hsz %Φ (Hmodel & HΨ & Hfn) HΦ".
     match goal with |- context [big_opL bi_sep ?Ξ' _] => set Ξ := Ξ' end.
     pose (Ψ' i acc vs_done := (
       Ψ i acc vs_done ∗
@@ -1032,14 +1035,13 @@ Section heapGS.
   Qed.
 
   Lemma chunk_foldr_spec_atomic Ψ l sz fn acc :
-    (0 ≤ sz)%Z →
     {{{
-      Ψ (Z.to_nat sz) acc None [] ∗
+      ▷ Ψ (Z.to_nat sz) acc None [] ∗
       □ (
         ∀ i acc vs,
         ⌜(S i + length vs)%nat = Z.to_nat sz⌝ -∗
         Ψ (S i) acc None vs -∗
-        chunk_au_load l i (λ v,
+        chunk_au_load l i (λ v, ▷
           Ψ (S i) acc (Some v) vs
         )
       ) ∗
@@ -1047,7 +1049,7 @@ Section heapGS.
         ∀ i v acc vs,
         ⌜(S i + length vs)%nat = Z.to_nat sz⌝ -∗
         Ψ (S i) acc (Some v) vs -∗
-        WP fn v acc {{ acc,
+        WP fn v acc {{ acc, ▷
           Ψ i acc None (v :: vs)
         }}
       )
@@ -1059,21 +1061,21 @@ Section heapGS.
       Ψ 0 acc None vs
     }}}.
   Proof.
-    iIntros "%Hsz %Φ (HΨ & #Hau & #Hfn) HΦ".
+    iIntros "%Φ (HΨ & #Hau & #Hfn) HΦ".
     wp_rec.
-    wp_smart_apply (chunk_foldri_spec_atomic Ψ with "[$HΨ $Hau] HΦ"); first done.
+    wp_smart_apply (chunk_foldri_spec_atomic Ψ with "[$HΨ $Hau] HΦ").
     iSmash.
   Qed.
   Lemma chunk_foldr_spec Ψ l dq vs (sz : Z) fn acc :
-    sz = length vs →
+    Z.to_nat sz = length vs →
     {{{
       chunk_model l dq vs ∗
-      Ψ (Z.to_nat sz) acc [] ∗
+      ▷ Ψ (Z.to_nat sz) acc [] ∗
       □ (
         ∀ i v acc,
         ⌜vs !! i = Some v⌝ -∗
         Ψ (S i) acc (drop (S i) vs) -∗
-        WP fn v acc {{ acc,
+        WP fn v acc {{ acc, ▷
           Ψ i acc (v :: drop (S i) vs)
         }}
       )
@@ -1091,14 +1093,14 @@ Section heapGS.
     iSmash.
   Qed.
   Lemma chunk_foldr_spec' Ψ l dq vs (sz : Z) fn acc :
-    sz = length vs →
+    Z.to_nat sz = length vs →
     {{{
       chunk_model l dq vs ∗
-      Ψ (Z.to_nat sz) acc [] ∗
+      ▷ Ψ (Z.to_nat sz) acc [] ∗
       ( [∗ list] i ↦ v ∈ vs,
         ∀ acc,
         Ψ (S i) acc (drop (S i) vs) -∗
-        WP fn v acc {{ acc,
+        WP fn v acc {{ acc, ▷
           Ψ i acc (v :: drop (S i) vs)
         }}
       )
@@ -1118,14 +1120,13 @@ Section heapGS.
   Qed.
 
   Lemma chunk_iteri_spec_atomic Ψ l sz fn :
-    (0 ≤ sz)%Z →
     {{{
-      Ψ 0 [] None ∗
+      ▷ Ψ 0 [] None ∗
       □ (
         ∀ i vs,
         ⌜i < Z.to_nat sz ∧ i = length vs⌝ -∗
         Ψ i vs None -∗
-        chunk_au_load l i (λ v,
+        chunk_au_load l i (λ v, ▷
           Ψ i vs (Some v)
         )
       ) ∗
@@ -1133,7 +1134,7 @@ Section heapGS.
         ∀ i vs v,
         ⌜i < Z.to_nat sz ∧ i = length vs⌝ -∗
         Ψ i vs (Some v) -∗
-        WP fn #i v {{ _,
+        WP fn #i v {{ _, ▷
           Ψ (S i) (vs ++ [v]) None
         }}
       )
@@ -1145,27 +1146,27 @@ Section heapGS.
       Ψ (Z.to_nat sz) vs None
     }}}.
   Proof.
-    iIntros "%Hsz %Φ (HΨ & #Hau & #Hfn) HΦ".
+    iIntros "%Φ (HΨ & #Hau & #Hfn) HΦ".
     wp_rec.
     pose Ψ' i vs o acc := (
       ⌜acc = #()⌝ ∗
       Ψ i vs o
     )%I.
-    wp_smart_apply (chunk_foldli_spec_atomic Ψ' with "[$HΨ]"); [done | | iSmash].
+    wp_smart_apply (chunk_foldli_spec_atomic Ψ' with "[$HΨ]"); last iSmash.
     repeat iSplit; try iSmash. iIntros "!> %i %vs %acc (%Hi& %Hi2) (-> & HΨ)".
     iApply (atomic_update_wand with "(Hau [//] HΨ)").
     iSmash.
   Qed.
   Lemma chunk_iteri_spec Ψ l dq vs (sz : Z) fn :
-    sz = length vs →
+    Z.to_nat sz = length vs →
     {{{
       chunk_model l dq vs ∗
-      Ψ 0 [] ∗
+      ▷ Ψ 0 [] ∗
       □ (
         ∀ i v,
         ⌜vs !! i = Some v⌝ -∗
         Ψ i (take i vs) -∗
-        WP fn #i v {{ _,
+        WP fn #i v {{ _, ▷
           Ψ (S i) (take i vs ++ [v])
         }}
       )
@@ -1186,13 +1187,13 @@ Section heapGS.
     wp_smart_apply (chunk_foldli_spec Ψ' with "[$Hmodel $HΨ]"); [done | iSmash..].
   Qed.
   Lemma chunk_iteri_spec' Ψ l dq vs (sz : Z) fn :
-    sz = length vs →
+    Z.to_nat sz = length vs →
     {{{
       chunk_model l dq vs ∗
-      Ψ 0 [] ∗
+      ▷ Ψ 0 [] ∗
       ( [∗ list] i ↦ v ∈ vs,
         Ψ i (take i vs) -∗
-        WP fn #i v {{ _,
+        WP fn #i v {{ _, ▷
           Ψ (S i) (take i vs ++ [v])
         }}
       )
@@ -1215,13 +1216,13 @@ Section heapGS.
     iSmash.
   Qed.
   Lemma chunk_iteri_spec_disentangled Ψ l dq vs (sz : Z) fn :
-    sz = length vs →
+    Z.to_nat sz = length vs →
     {{{
       chunk_model l dq vs ∗
       □ (
         ∀ i v,
         ⌜vs !! i = Some v⌝ -∗
-        WP fn #i v {{ _,
+        WP fn #i v {{ _, ▷
           Ψ i v
         }}
       )
@@ -1245,11 +1246,11 @@ Section heapGS.
     eapply Nat.lt_le_incl, lookup_lt_Some. done.
   Qed.
   Lemma chunk_iteri_spec_disentangled' Ψ l dq vs (sz : Z) fn :
-    sz = length vs →
+    Z.to_nat sz = length vs →
     {{{
       chunk_model l dq vs ∗
       ( [∗ list] i ↦ v ∈ vs,
-        WP fn #i v {{ _,
+        WP fn #i v {{ _, ▷
           Ψ i v
         }}
       )
@@ -1275,14 +1276,13 @@ Section heapGS.
   Qed.
 
   Lemma chunk_iter_spec_atomic Ψ l sz fn :
-    (0 ≤ sz)%Z →
     {{{
-      Ψ 0 [] None ∗
+      ▷ Ψ 0 [] None ∗
       □ (
         ∀ i vs,
         ⌜i < Z.to_nat sz ∧ i = length vs⌝ -∗
         Ψ i vs None -∗
-        chunk_au_load l i (λ v,
+        chunk_au_load l i (λ v, ▷
           Ψ i vs (Some v)
         )
       ) ∗
@@ -1290,7 +1290,7 @@ Section heapGS.
         ∀ i vs v,
         ⌜i < Z.to_nat sz ∧ i = length vs⌝ -∗
         Ψ i vs (Some v) -∗
-        WP fn v {{ _,
+        WP fn v {{ _, ▷
           Ψ (S i) (vs ++ [v]) None
         }}
       )
@@ -1302,21 +1302,21 @@ Section heapGS.
       Ψ (Z.to_nat sz) vs None
     }}}.
   Proof.
-    iIntros "%Hsz %Φ (HΨ & #Hau & #Hfn) HΦ".
+    iIntros "%Φ (HΨ & #Hau & #Hfn) HΦ".
     wp_rec.
-    wp_smart_apply (chunk_iteri_spec_atomic Ψ with "[$HΨ $Hau] HΦ"); first done.
+    wp_smart_apply (chunk_iteri_spec_atomic Ψ with "[$HΨ $Hau] HΦ").
     iSmash.
   Qed.
   Lemma chunk_iter_spec Ψ l dq vs (sz : Z) fn :
-    sz = length vs →
+    Z.to_nat sz = length vs →
     {{{
       chunk_model l dq vs ∗
-      Ψ 0 [] ∗
+      ▷ Ψ 0 [] ∗
       □ (
         ∀ i v,
         ⌜vs !! i = Some v⌝ -∗
         Ψ i (take i vs) -∗
-        WP fn v {{ _,
+        WP fn v {{ _, ▷
           Ψ (S i) (take i vs ++ [v])
         }}
       )
@@ -1334,13 +1334,13 @@ Section heapGS.
     iSmash.
   Qed.
   Lemma chunk_iter_spec' Ψ l dq vs (sz : Z) fn :
-    sz = length vs →
+    Z.to_nat sz = length vs →
     {{{
       chunk_model l dq vs ∗
-      Ψ 0 [] ∗
+      ▷ Ψ 0 [] ∗
       ( [∗ list] i ↦ v ∈ vs,
         Ψ i (take i vs) -∗
-        WP fn v {{ _,
+        WP fn v {{ _, ▷
           Ψ (S i) (take i vs ++ [v])
         }}
       )
@@ -1359,13 +1359,13 @@ Section heapGS.
     iSmash.
   Qed.
   Lemma chunk_iter_spec_disentangled Ψ l dq vs (sz : Z) fn :
-    sz = length vs →
+    Z.to_nat sz = length vs →
     {{{
       chunk_model l dq vs ∗
       □ (
         ∀ i v,
         ⌜vs !! i = Some v⌝ -∗
-        WP fn v {{ _,
+        WP fn v {{ _, ▷
           Ψ i v
         }}
       )
@@ -1385,11 +1385,11 @@ Section heapGS.
     iSmash.
   Qed.
   Lemma chunk_iter_spec_disentangled' Ψ l dq vs (sz : Z) fn :
-    sz = length vs →
+    Z.to_nat sz = length vs →
     {{{
       chunk_model l dq vs ∗
       ( [∗ list] i ↦ v ∈ vs,
-        WP fn v {{ _,
+        WP fn v {{ _, ▷
           Ψ i v
         }}
       )
@@ -1411,14 +1411,13 @@ Section heapGS.
   Qed.
 
   Lemma chunk_applyi_spec_atomic Ψ l sz fn :
-    (0 ≤ sz)%Z →
     {{{
-      Ψ 0 [] None [] ∗
+      ▷ Ψ 0 [] None [] ∗
       □ (
         ∀ i vs ws,
         ⌜i < Z.to_nat sz ∧ i = length vs ∧ length vs = length ws⌝ -∗
         Ψ i vs None ws -∗
-        chunk_au_load l i (λ v,
+        chunk_au_load l i (λ v, ▷
           Ψ i vs (Some $ inl v) ws
         )
       ) ∗
@@ -1426,7 +1425,7 @@ Section heapGS.
         ∀ i vs v ws,
         ⌜i < Z.to_nat sz ∧ i = length vs ∧ length vs = length ws⌝ -∗
         Ψ i vs (Some $ inl v) ws -∗
-        WP fn #i v {{ w,
+        WP fn #i v {{ w, ▷
           Ψ i vs (Some $ inr (v, w)) ws
         }}
       ) ∗
@@ -1434,7 +1433,7 @@ Section heapGS.
         ∀ i vs v ws w,
         ⌜i < Z.to_nat sz ∧ i = length vs ∧ length vs = length ws⌝ -∗
         Ψ i vs (Some $ inr (v, w)) ws -∗
-        chunk_au_store l i w (
+        chunk_au_store l i w ( ▷
           Ψ (S i) (vs ++ [v]) None (ws ++ [w])
         )
       )
@@ -1446,14 +1445,14 @@ Section heapGS.
       Ψ (Z.to_nat sz) vs None ws
     }}}.
   Proof.
-    iIntros "%Hsz %Φ (HΨ & #Hau1 & #Hfn & #Hau2) HΦ".
+    iIntros "%Φ (HΨ & #Hau1 & #Hfn & #Hau2) HΦ".
     wp_rec.
     pose (Ψ' i vs o := (
       ∃ ws,
       ⌜length vs = length ws⌝ ∗
       Ψ i vs (inl <$> o) ws
     )%I).
-    wp_smart_apply (chunk_iteri_spec_atomic Ψ' with "[HΨ]"); [done | | iSmash].
+    wp_smart_apply (chunk_iteri_spec_atomic Ψ' with "[HΨ]"); last iSmash.
     iSplitL "HΨ". { iExists []. iSmash. }
     iSplit; iIntros "!> %i %vs".
     - iIntros "(%Hi1 & %Hi2) (%ws & %Hws & HΨ)".
@@ -1469,15 +1468,15 @@ Section heapGS.
       rewrite !app_length. iSmash.
   Qed.
   Lemma chunk_applyi_spec Ψ l vs (sz : Z) fn :
-    sz = length vs →
+    Z.to_nat sz = length vs →
     {{{
       chunk_model l (DfracOwn 1) vs ∗
-      Ψ 0 [] [] ∗
+      ▷ Ψ 0 [] [] ∗
       □ (
         ∀ i v ws,
         ⌜i = length ws ∧ vs !! i = Some v⌝ -∗
         Ψ i (take i vs) ws -∗
-        WP fn #i v {{ w,
+        WP fn #i v {{ w, ▷
           Ψ (S i) (take i vs ++ [v]) (ws ++ [w])
         }}
       )
@@ -1490,7 +1489,7 @@ Section heapGS.
       Ψ (Z.to_nat sz) vs ws
     }}}.
   Proof.
-    iIntros (->) "%Φ (Hmodel & HΨ & #Hfn) HΦ".
+    iIntros "%Hsz %Φ (Hmodel & HΨ & #Hfn) HΦ".
     pose (Ψ' i vs_done o ws := (
       ⌜vs_done = take i vs⌝ ∗
       chunk_model l (DfracOwn 1) (ws ++ drop i vs) ∗
@@ -1505,9 +1504,9 @@ Section heapGS.
           Ψ (S i) (vs_done ++ [v]) (ws ++ [w])
       end
     )%I).
-    wp_apply (chunk_applyi_spec_atomic Ψ' with "[$Hmodel $HΨ]"); first lia; last first.
+    wp_apply (chunk_applyi_spec_atomic Ψ' with "[$Hmodel $HΨ]"); last first.
     { iIntros "%vs_done %ws ((%Hvs_done_1 & %Hws) & (-> & Hmodel & HΨ))".
-      rewrite Nat2Z.id firstn_all2; last lia. rewrite skipn_all2; last lia. rewrite right_id.
+      rewrite Hsz firstn_all2; last lia. rewrite skipn_all2; last lia. rewrite right_id.
       iApply ("HΦ" $! ws). iSmash.
     }
     iSplit; first iSmash. repeat iSplit.
@@ -1538,15 +1537,15 @@ Section heapGS.
       rewrite Hi Hws Nat.sub_diag -assoc //.
   Qed.
   Lemma chunk_applyi_spec' Ψ l vs (sz : Z) fn :
-    sz = length vs →
+    Z.to_nat sz = length vs →
     {{{
       chunk_model l (DfracOwn 1) vs ∗
-      Ψ 0 [] [] ∗
+      ▷ Ψ 0 [] [] ∗
       ( [∗ list] i ↦ v ∈ vs,
         ∀ ws,
         ⌜i = length ws⌝ -∗
         Ψ i (take i vs) ws -∗
-        WP fn #i v {{ w,
+        WP fn #i v {{ w, ▷
           Ψ (S i) (take i vs ++ [v]) (ws ++ [w])
         }}
       )
@@ -1574,13 +1573,13 @@ Section heapGS.
     setoid_rewrite Nat.add_succ_r. iSmash.
   Qed.
   Lemma chunk_applyi_spec_disentangled Ψ l vs (sz : Z) fn :
-    sz = length vs →
+    Z.to_nat sz = length vs →
     {{{
       chunk_model l (DfracOwn 1) vs ∗
       □ (
         ∀ i v,
         ⌜vs !! i = Some v⌝ -∗
-        WP fn #i v {{ w,
+        WP fn #i v {{ w, ▷
           Ψ i w
         }}
       )
@@ -1604,11 +1603,11 @@ Section heapGS.
     rewrite big_sepL_snoc. iSmash.
   Qed.
   Lemma chunk_applyi_spec_disentangled' Ψ l vs (sz : Z) fn :
-    sz = length vs →
+    Z.to_nat sz = length vs →
     {{{
       chunk_model l (DfracOwn 1) vs ∗
       ( [∗ list] i ↦ v ∈ vs,
-        WP fn #i v {{ w,
+        WP fn #i v {{ w, ▷
           Ψ i w
         }}
       )
@@ -1633,14 +1632,13 @@ Section heapGS.
   Qed.
 
   Lemma chunk_apply_spec_atomic Ψ l sz fn :
-    (0 ≤ sz)%Z →
     {{{
-      Ψ 0 [] None [] ∗
+      ▷ Ψ 0 [] None [] ∗
       □ (
         ∀ i vs ws,
         ⌜i < Z.to_nat sz ∧ i = length vs ∧ length vs = length ws⌝ -∗
         Ψ i vs None ws -∗
-        chunk_au_load l i (λ v,
+        chunk_au_load l i (λ v, ▷
           Ψ i vs (Some $ inl v) ws
         )
       ) ∗
@@ -1648,7 +1646,7 @@ Section heapGS.
         ∀ i vs v ws,
         ⌜i < Z.to_nat sz ∧ i = length vs ∧ length vs = length ws⌝ -∗
         Ψ i vs (Some $ inl v) ws -∗
-        WP fn v {{ w,
+        WP fn v {{ w, ▷
           Ψ i vs (Some $ inr (v, w)) ws
         }}
       ) ∗
@@ -1656,7 +1654,7 @@ Section heapGS.
         ∀ i vs v ws w,
         ⌜i < Z.to_nat sz ∧ i = length vs ∧ length vs = length ws⌝ -∗
         Ψ i vs (Some $ inr (v, w)) ws -∗
-        chunk_au_store l i w (
+        chunk_au_store l i w ( ▷
           Ψ (S i) (vs ++ [v]) None (ws ++ [w])
         )
       )
@@ -1668,22 +1666,22 @@ Section heapGS.
       Ψ (Z.to_nat sz) vs None ws
     }}}.
   Proof.
-    iIntros "%Hsz %Φ (HΨ & #Hau1 & #Hfn & #Hau2) HΦ".
+    iIntros "%Φ (HΨ & #Hau1 & #Hfn & #Hau2) HΦ".
     wp_rec.
-    wp_smart_apply (chunk_applyi_spec_atomic Ψ with "[$HΨ $Hau1 $Hau2] HΦ"); first done. iIntros "!> %i %vs %v %ws (%Hi1 & %Hi2 & %Hws) HΨ".
+    wp_smart_apply (chunk_applyi_spec_atomic Ψ with "[$HΨ $Hau1 $Hau2] HΦ"). iIntros "!> %i %vs %v %ws (%Hi1 & %Hi2 & %Hws) HΨ".
     wp_smart_apply (wp_wand with "(Hfn [//] HΨ)").
     iSmash.
   Qed.
   Lemma chunk_apply_spec Ψ l vs (sz : Z) fn :
-    sz = length vs →
+    Z.to_nat sz = length vs →
     {{{
       chunk_model l (DfracOwn 1) vs ∗
-      Ψ 0 [] [] ∗
+      ▷ Ψ 0 [] [] ∗
       □ (
         ∀ i v ws,
         ⌜i = length ws ∧ vs !! i = Some v⌝ -∗
         Ψ i (take i vs) ws -∗
-        WP fn v {{ w,
+        WP fn v {{ w, ▷
           Ψ (S i) (take i vs ++ [v]) (ws ++ [w])
         }}
       )
@@ -1698,19 +1696,19 @@ Section heapGS.
   Proof.
     iIntros "%Hsz %Φ (Hmodel & HΨ & #Hfn) HΦ".
     wp_rec.
-    wp_smart_apply (chunk_applyi_spec Ψ with "[$Hmodel $HΨ] HΦ"); first done.
-    iSmash.
+    wp_smart_apply (chunk_applyi_spec Ψ with "[$Hmodel $HΨ] HΦ"); first done. iIntros "!> %i %v %ws (%Hi & %Hlookup) HΨ".
+    wp_smart_apply ("Hfn" with "[//] HΨ").
   Qed.
   Lemma chunk_apply_spec' Ψ l vs (sz : Z) fn :
-    sz = length vs →
+    Z.to_nat sz = length vs →
     {{{
       chunk_model l (DfracOwn 1) vs ∗
-      Ψ 0 [] [] ∗
+      ▷ Ψ 0 [] [] ∗
       ( [∗ list] i ↦ v ∈ vs,
         ∀ ws,
         ⌜i = length ws⌝ -∗
         Ψ i (take i vs) ws -∗
-        WP fn v {{ w,
+        WP fn v {{ w, ▷
           Ψ (S i) (take i vs ++ [v]) (ws ++ [w])
         }}
       )
@@ -1730,13 +1728,13 @@ Section heapGS.
     iSmash.
   Qed.
   Lemma chunk_apply_spec_disentangled Ψ l vs (sz : Z) fn :
-    sz = length vs →
+    Z.to_nat sz = length vs →
     {{{
       chunk_model l (DfracOwn 1) vs ∗
       □ (
         ∀ i v,
         ⌜vs !! i = Some v⌝ -∗
-        WP fn v {{ w,
+        WP fn v {{ w, ▷
           Ψ i w
         }}
       )
@@ -1757,11 +1755,11 @@ Section heapGS.
     iSmash.
   Qed.
   Lemma chunk_apply_spec_disentangled' Ψ l vs (sz : Z) fn :
-    sz = length vs →
+    Z.to_nat sz = length vs →
     {{{
       chunk_model l (DfracOwn 1) vs ∗
       ( [∗ list] i ↦ v ∈ vs,
-        WP fn v {{ w,
+        WP fn v {{ w, ▷
           Ψ i w
         }}
       )
@@ -1783,14 +1781,13 @@ Section heapGS.
   Qed.
 
   Lemma chunk_initi_spec Ψ sz fn :
-    (0 ≤ sz)%Z →
     {{{
-      Ψ 0 [] ∗
+      ▷ Ψ 0 [] ∗
       □ (
         ∀ i vs,
         ⌜i < Z.to_nat sz ∧ i = length vs⌝ -∗
         Ψ i vs -∗
-        WP fn #i {{ v,
+        WP fn #i {{ v, ▷
           Ψ (S i) (vs ++ [v])
         }}
       )
@@ -1804,9 +1801,9 @@ Section heapGS.
       if decide (0 < sz)%Z then meta_token l ⊤ else True
     }}}.
   Proof.
-    iIntros "%Hsz %Φ (HΨ & #Hfn) HΦ".
+    iIntros "%Φ (HΨ & #Hfn) HΦ".
     wp_rec.
-    wp_smart_apply (chunk_make_spec with "[//]"); first done. iIntros "%l (Hmodel & Hmeta)".
+    wp_smart_apply (chunk_make_spec with "[//]"). iIntros "%l (Hmodel & Hmeta)".
     pose Ψ' i vs' vs := (
       Ψ i vs
     )%I.
@@ -1822,14 +1819,13 @@ Section heapGS.
     iSmash.
   Qed.
   Lemma chunk_initi_spec' Ψ sz fn :
-    (0 ≤ sz)%Z →
     {{{
-      Ψ 0 [] ∗
+      ▷ Ψ 0 [] ∗
       ( [∗ list] i ∈ seq 0 (Z.to_nat sz),
         ∀ vs,
         ⌜i = length vs⌝ -∗
         Ψ i vs -∗
-        WP fn #i {{ v,
+        WP fn #i {{ v, ▷
           Ψ (S i) (vs ++ [v])
         }}
       )
@@ -1843,13 +1839,13 @@ Section heapGS.
       if decide (0 < sz)%Z then meta_token l ⊤ else True
     }}}.
   Proof.
-    iIntros "%Hsz %Φ (HΨ & Hfn) HΦ".
+    iIntros "%Φ (HΨ & Hfn) HΦ".
     match goal with |- context [big_opL bi_sep (λ _, ?Ξ') _] => set Ξ := Ξ' end.
     pose (Ψ' i vs := (
       Ψ i vs ∗
       [∗ list] j ∈ seq i (Z.to_nat sz - i), Ξ j
     )%I).
-    wp_apply (chunk_initi_spec Ψ' with "[$HΨ Hfn]"); [done | | iSmash].
+    wp_apply (chunk_initi_spec Ψ' with "[$HΨ Hfn]"); last iSmash.
     rewrite Nat.sub_0_r. iFrame. iIntros "!> %i %vs (%Hi1 & %Hi2) (HΨ & HΞ)".
     destruct (Nat.lt_exists_pred 0 (Z.to_nat sz - i)) as (k & Hk & _); first lia. rewrite Hk.
     rewrite -cons_seq. iDestruct "HΞ" as "(Hfn & HΞ)".
@@ -1857,12 +1853,11 @@ Section heapGS.
     rewrite Nat.sub_succ_r Hk //.
   Qed.
   Lemma chunk_initi_spec_disentangled Ψ sz fn :
-    (0 ≤ sz)%Z →
     {{{
       □ (
         ∀ i,
         ⌜i < Z.to_nat sz⌝ -∗
-        WP fn #i {{ v,
+        WP fn #i {{ v, ▷
           Ψ i v
         }}
       )
@@ -1878,19 +1873,18 @@ Section heapGS.
       if decide (0 < sz)%Z then meta_token l ⊤ else True
     }}}.
   Proof.
-    iIntros "%Hsz %Φ #Hfn HΦ".
+    iIntros "%Φ #Hfn HΦ".
     pose (Ψ' i vs := (
       [∗ list] j ↦ v ∈ vs, Ψ j v
     )%I).
-    wp_apply (chunk_initi_spec Ψ'); [done | | iSmash].
+    wp_apply (chunk_initi_spec Ψ'); last iSmash.
     rewrite /Ψ'. iSteps.
     rewrite big_sepL_snoc. iSmash.
   Qed.
   Lemma chunk_initi_spec_disentangled' Ψ sz fn :
-    (0 ≤ sz)%Z →
     {{{
       ( [∗ list] i ∈ seq 0 (Z.to_nat sz),
-        WP fn #i {{ v,
+        WP fn #i {{ v, ▷
           Ψ i v
         }}
       )
@@ -1906,25 +1900,24 @@ Section heapGS.
       if decide (0 < sz)%Z then meta_token l ⊤ else True
     }}}.
   Proof.
-    iIntros "%Hsz %Φ Hfn HΦ".
+    iIntros "%Φ Hfn HΦ".
     pose (Ψ' i vs := (
       [∗ list] j ↦ v ∈ vs, Ψ j v
     )%I).
-    wp_apply (chunk_initi_spec' Ψ' with "[Hfn]"); [done | | iSmash].
+    wp_apply (chunk_initi_spec' Ψ' with "[Hfn]"); last iSmash.
     rewrite /Ψ'. iSteps.
     iApply (big_sepL_impl with "Hfn"). iSteps.
     rewrite big_sepL_snoc. iSmash.
   Qed.
 
   Lemma chunk_init_spec Ψ sz fn :
-    (0 ≤ sz)%Z →
     {{{
-      Ψ 0 [] ∗
+      ▷ Ψ 0 [] ∗
       □ (
         ∀ i vs,
         ⌜i < Z.to_nat sz ∧ i = length vs⌝ -∗
         Ψ i vs -∗
-        WP fn #() {{ v,
+        WP fn #() {{ v, ▷
           Ψ (S i) (vs ++ [v])
         }}
       )
@@ -1938,20 +1931,19 @@ Section heapGS.
       if decide (0 < sz)%Z then meta_token l ⊤ else True
     }}}.
   Proof.
-    iIntros "%Hsz %Φ (HΨ & #Hfn) HΦ".
+    iIntros "%Φ (HΨ & #Hfn) HΦ".
     wp_rec.
-    wp_smart_apply (chunk_initi_spec Ψ with "[$HΨ] HΦ"); first done.
+    wp_smart_apply (chunk_initi_spec Ψ with "[$HΨ] HΦ").
     iSmash.
   Qed.
   Lemma chunk_init_spec' Ψ sz fn :
-    (0 ≤ sz)%Z →
     {{{
-      Ψ 0 [] ∗
+      ▷ Ψ 0 [] ∗
       ( [∗ list] i ∈ seq 0 (Z.to_nat sz),
         ∀ vs,
         ⌜i = length vs⌝ -∗
         Ψ i vs -∗
-        WP fn #() {{ v,
+        WP fn #() {{ v, ▷
           Ψ (S i) (vs ++ [v])
         }}
       )
@@ -1965,19 +1957,18 @@ Section heapGS.
       if decide (0 < sz)%Z then meta_token l ⊤ else True
     }}}.
   Proof.
-    iIntros "%Hsz %Φ (HΨ & Hfn) HΦ".
+    iIntros "%Φ (HΨ & Hfn) HΦ".
     wp_rec.
-    wp_smart_apply (chunk_initi_spec' Ψ with "[$HΨ Hfn] HΦ"); first done.
+    wp_smart_apply (chunk_initi_spec' Ψ with "[$HΨ Hfn] HΦ").
     iApply (big_sepL_impl with "Hfn").
     iSmash.
   Qed.
   Lemma chunk_init_spec_disentangled Ψ sz fn :
-    (0 ≤ sz)%Z →
     {{{
       □ (
         ∀ i,
         ⌜i < Z.to_nat sz⌝ -∗
-        WP fn #() {{ v,
+        WP fn #() {{ v, ▷
           Ψ i v
         }}
       )
@@ -1993,16 +1984,15 @@ Section heapGS.
       if decide (0 < sz)%Z then meta_token l ⊤ else True
     }}}.
   Proof.
-    iIntros "%Hsz %Φ #Hfn HΦ".
+    iIntros "%Φ #Hfn HΦ".
     wp_rec.
-    wp_smart_apply (chunk_initi_spec_disentangled Ψ with "[] HΦ"); first done.
+    wp_smart_apply (chunk_initi_spec_disentangled Ψ with "[] HΦ").
     iSmash.
   Qed.
   Lemma chunk_init_spec_disentangled' Ψ sz fn :
-    (0 ≤ sz)%Z →
     {{{
       ( [∗ list] i ∈ seq 0 (Z.to_nat sz),
-        WP fn #() {{ v,
+        WP fn #() {{ v, ▷
           Ψ i v
         }}
       )
@@ -2018,22 +2008,21 @@ Section heapGS.
       if decide (0 < sz)%Z then meta_token l ⊤ else True
     }}}.
   Proof.
-    iIntros "%Hsz %Φ Hfn HΦ".
+    iIntros "%Φ Hfn HΦ".
     wp_rec.
-    wp_smart_apply (chunk_initi_spec_disentangled' Ψ with "[Hfn] HΦ"); first done.
+    wp_smart_apply (chunk_initi_spec_disentangled' Ψ with "[Hfn] HΦ").
     iApply (big_sepL_impl with "Hfn").
     iSmash.
   Qed.
 
   Lemma chunk_mapi_spec_atomic Ψ l sz fn :
-    (0 ≤ sz)%Z →
     {{{
-      Ψ 0 [] None [] ∗
+      ▷ Ψ 0 [] None [] ∗
       □ (
         ∀ i vs ws,
         ⌜i < Z.to_nat sz ∧ i = length vs ∧ length vs = length ws⌝ -∗
         Ψ i vs None ws -∗
-        chunk_au_load l i (λ v,
+        chunk_au_load l i (λ v, ▷
           Ψ i vs (Some v) ws
         )
       ) ∗
@@ -2041,7 +2030,7 @@ Section heapGS.
         ∀ i vs v ws,
         ⌜i < Z.to_nat sz ∧ i = length vs ∧ length vs = length ws⌝ -∗
         Ψ i vs (Some v) ws -∗
-        WP fn #i v {{ w,
+        WP fn #i v {{ w, ▷
           Ψ (S i) (vs ++ [v]) None (ws ++ [w])
         }}
       )
@@ -2055,37 +2044,38 @@ Section heapGS.
       if decide (0 < sz)%Z then meta_token l' ⊤ else True
     }}}.
   Proof.
-    iIntros "%Hsz %Φ (HΨ & #Hau & #Hfn) HΦ".
+    iIntros "%Φ (HΨ & #Hau & #Hfn) HΦ".
     wp_rec.
     pose Ψ' i ws := (
       ∃ vs,
       ⌜length vs = length ws⌝ ∗
       Ψ i vs None ws
     )%I.
-    wp_smart_apply (chunk_initi_spec Ψ' with "[HΨ]"); first done; last first.
+    wp_smart_apply (chunk_initi_spec Ψ' with "[HΨ]"); last first.
     { iIntros "%l' %ws (%Hws & Hmodel & (%vs & %Hvs & HΨ) & Hmeta)".
       iApply ("HΦ" with "[$Hmodel $HΨ $Hmeta]").
       iSmash.
     }
     iSplit. { iExists []. iSmash. }
     iIntros "!> %i %ws (%Hi1 & %Hi2) (%vs & %Hvs & HΨ)".
-    wp_pures. wp_bind (!_)%E.
+    wp_pure credit:"H£". wp_pures. wp_bind (!_)%E.
     iMod ("Hau" with "[] HΨ") as "(%dq & %v & H↦ & _ & HΨ)"; first iSmash.
     wp_load.
     iMod ("HΨ" with "H↦") as "HΨ". iModIntro.
+    iMod (lc_fupd_elim_later with "H£ HΨ") as "HΨ".
     wp_apply (wp_wand with "(Hfn [] HΨ)"); first iSmash. iIntros "%w HΨ".
     iExists (vs ++ [v]). iFrame. rewrite !app_length. iSmash.
   Qed.
   Lemma chunk_mapi_spec Ψ l dq vs (sz : Z) fn :
-    sz = length vs →
+    Z.to_nat sz = length vs →
     {{{
       chunk_model l dq vs ∗
-      Ψ 0 [] [] ∗
+      ▷ Ψ 0 [] [] ∗
       □ (
         ∀ i v ws,
         ⌜vs !! i = Some v ∧ i = length ws⌝ -∗
         Ψ i (take i vs) ws -∗
-        WP fn #i v {{ w,
+        WP fn #i v {{ w, ▷
           Ψ (S i) (take i vs ++ [v]) (ws ++ [w])
         }}
       )
@@ -2120,18 +2110,17 @@ Section heapGS.
       feed pose proof (list_lookup_lookup_total_lt vs i); first lia.
       wp_apply (wp_wand with "(Hfn [] HΨ)"); first iSmash. iIntros "%w HΨ". iFrame.
       erewrite take_S_r; done.
-    - lia.
   Qed.
   Lemma chunk_mapi_spec' Ψ l dq vs (sz : Z) fn :
-    sz = length vs →
+    Z.to_nat sz = length vs →
     {{{
       chunk_model l dq vs ∗
-      Ψ 0 [] [] ∗
+      ▷ Ψ 0 [] [] ∗
       ( [∗ list] i ↦ v ∈ vs,
         ∀ ws,
         ⌜i = length ws⌝ -∗
         Ψ i (take i vs) ws -∗
-        WP fn #i v {{ w,
+        WP fn #i v {{ w, ▷
           Ψ (S i) (take i vs ++ [v]) (ws ++ [w])
         }}
       )
@@ -2160,13 +2149,13 @@ Section heapGS.
     setoid_rewrite Nat.add_succ_r. iSmash.
   Qed.
   Lemma chunk_mapi_spec_disentangled Ψ l dq vs (sz : Z) fn :
-    sz = length vs →
+    Z.to_nat sz = length vs →
     {{{
       chunk_model l dq vs ∗
       □ (
         ∀ i v,
         ⌜vs !! i = Some v⌝ -∗
-        WP fn #i v {{ w,
+        WP fn #i v {{ w, ▷
           Ψ i v w
         }}
       )
@@ -2192,11 +2181,11 @@ Section heapGS.
     eapply Nat.lt_le_incl, lookup_lt_Some. done.
   Qed.
   Lemma chunk_mapi_spec_disentangled' Ψ l dq vs (sz : Z) fn :
-    sz = length vs →
+    Z.to_nat sz = length vs →
     {{{
       chunk_model l dq vs ∗
       ( [∗ list] i ↦ v ∈ vs,
-        WP fn #i v {{ w,
+        WP fn #i v {{ w, ▷
           Ψ i v w
         }}
       )
@@ -2227,14 +2216,13 @@ Section heapGS.
   Qed.
 
   Lemma chunk_map_spec_atomic Ψ l sz fn :
-    (0 ≤ sz)%Z →
     {{{
-      Ψ 0 [] None [] ∗
+      ▷ Ψ 0 [] None [] ∗
       □ (
         ∀ i vs ws,
         ⌜i < Z.to_nat sz ∧ i = length vs ∧ length vs = length ws⌝ -∗
         Ψ i vs None ws -∗
-        chunk_au_load l i (λ v,
+        chunk_au_load l i (λ v, ▷
           Ψ i vs (Some v) ws
         )
       ) ∗
@@ -2242,7 +2230,7 @@ Section heapGS.
         ∀ i vs v ws,
         ⌜i < Z.to_nat sz ∧ i = length vs ∧ length vs = length ws⌝ -∗
         Ψ i vs (Some v) ws -∗
-        WP fn v {{ w,
+        WP fn v {{ w, ▷
           Ψ (S i) (vs ++ [v]) None (ws ++ [w])
         }}
       )
@@ -2256,21 +2244,21 @@ Section heapGS.
       if decide (0 < sz)%Z then meta_token l' ⊤ else True
     }}}.
   Proof.
-    iIntros "%Hsz %Φ (HΨ & #Hau & #Hfn) HΦ".
+    iIntros "%Φ (HΨ & #Hau & #Hfn) HΦ".
     wp_rec.
-    wp_smart_apply (chunk_mapi_spec_atomic Ψ with "[$HΨ $Hau] HΦ"); first done. iIntros "!> %i %vs %v %ws (%Hi1 & %Hi2 & %Hws) HΨ".
+    wp_smart_apply (chunk_mapi_spec_atomic Ψ with "[$HΨ $Hau] HΦ"). iIntros "!> %i %vs %v %ws (%Hi1 & %Hi2 & %Hws) HΨ".
     wp_smart_apply ("Hfn" with "[//] HΨ").
   Qed.
   Lemma chunk_map_spec Ψ l dq vs (sz : Z) fn :
-    sz = length vs →
+    Z.to_nat sz = length vs →
     {{{
       chunk_model l dq vs ∗
-      Ψ 0 [] [] ∗
+      ▷ Ψ 0 [] [] ∗
       □ (
         ∀ i v ws,
         ⌜vs !! i = Some v ∧ i = length ws⌝ -∗
         Ψ i (take i vs) ws -∗
-        WP fn v {{ w,
+        WP fn v {{ w, ▷
           Ψ (S i) (take i vs ++ [v]) (ws ++ [w])
         }}
       )
@@ -2290,15 +2278,15 @@ Section heapGS.
     iSmash.
   Qed.
   Lemma chunk_map_spec' Ψ l dq vs (sz : Z) fn :
-    sz = length vs →
+    Z.to_nat sz = length vs →
     {{{
       chunk_model l dq vs ∗
-      Ψ 0 [] [] ∗
+      ▷ Ψ 0 [] [] ∗
       ( [∗ list] i ↦ v ∈ vs,
         ∀ ws,
         ⌜i = length ws⌝ -∗
         Ψ i (take i vs) ws -∗
-        WP fn v {{ w,
+        WP fn v {{ w, ▷
           Ψ (S i) (take i vs ++ [v]) (ws ++ [w])
         }}
       )
@@ -2319,13 +2307,13 @@ Section heapGS.
     iSmash.
   Qed.
   Lemma chunk_map_spec_disentangled Ψ l dq vs (sz : Z) fn :
-    sz = length vs →
+    Z.to_nat sz = length vs →
     {{{
       chunk_model l dq vs ∗
       □ (
         ∀ i v,
         ⌜vs !! i = Some v⌝ -∗
-        WP fn v {{ w,
+        WP fn v {{ w, ▷
           Ψ i v w
         }}
       )
@@ -2347,11 +2335,11 @@ Section heapGS.
     iSmash.
   Qed.
   Lemma chunk_map_spec_disentangled' Ψ l dq vs (sz : Z) fn :
-    sz = length vs →
+    Z.to_nat sz = length vs →
     {{{
       chunk_model l dq vs ∗
       ( [∗ list] i ↦ v ∈ vs,
-        WP fn v {{ w,
+        WP fn v {{ w, ▷
           Ψ i v w
         }}
       )
@@ -2375,14 +2363,13 @@ Section heapGS.
   Qed.
 
   Lemma chunk_copy_spec_atomic Ψ l1 l2 sz :
-    (0 ≤ sz)%Z →
     {{{
-      Ψ 0 [] None ∗
+      ▷ Ψ 0 [] None ∗
       □ (
         ∀ i vs,
         ⌜i < Z.to_nat sz ∧ i = length vs⌝ -∗
         Ψ i vs None -∗
-        chunk_au_load l1 i (λ v,
+        chunk_au_load l1 i (λ v, ▷
           Ψ i vs (Some v)
         )
       ) ∗
@@ -2390,7 +2377,7 @@ Section heapGS.
         ∀ i vs v,
         ⌜i < Z.to_nat sz ∧ i = length vs⌝ -∗
         Ψ i vs (Some v) -∗
-        chunk_au_store l2 i v (
+        chunk_au_store l2 i v ( ▷
           Ψ (S i) (vs ++ [v]) None
         )
       )
@@ -2402,9 +2389,9 @@ Section heapGS.
       Ψ (Z.to_nat sz) vs None
     }}}.
   Proof.
-    iIntros "%Hsz %Φ (HΨ & #Hau1 & #Hau2) HΦ".
+    iIntros "%Φ (HΨ & #Hau1 & #Hau2) HΦ".
     wp_rec.
-    wp_smart_apply (chunk_iteri_spec_atomic Ψ with "[$HΨ]"); [done | | iSmash].
+    wp_smart_apply (chunk_iteri_spec_atomic Ψ with "[$HΨ]"); last iSmash.
     iSplit; first iSmash. iIntros "!> %i %vs %v (%Hi1 & %Hi2) HΨ".
     wp_pures.
     iMod ("Hau2" with "[] HΨ") as "(%v' & H↦ & _ & HΨ)"; first iSmash.
@@ -2412,8 +2399,8 @@ Section heapGS.
     iApply ("HΨ" with "H↦").
   Qed.
   Lemma chunk_copy_spec l1 dq1 vs1 (sz : Z) l2 vs2 :
-    sz = length vs1 →
-    sz = length vs2 →
+    Z.to_nat sz = length vs1 →
+    Z.to_nat sz = length vs2 →
     {{{
       chunk_model l1 dq1 vs1 ∗
       chunk_model l2 (DfracOwn 1) vs2
@@ -2432,7 +2419,7 @@ Section heapGS.
       chunk_model l2 (DfracOwn 1) (vs1_done ++ drop i vs2) ∗
       ⌜from_option (λ v1, vs1 !! i = Some v1) True o⌝
     )%I).
-    wp_apply (chunk_copy_spec_atomic Ψ with "[$Hmodel1 $Hmodel2]"); first lia; last first.
+    wp_apply (chunk_copy_spec_atomic Ψ with "[$Hmodel1 $Hmodel2]"); last first.
     { iIntros "%vs1_done (_ & (-> & Hmodel1 & Hmodel2 & _))".
       iApply ("HΦ" with "[$Hmodel1 Hmodel2]").
       rewrite firstn_all2; last lia. rewrite skipn_all2; last lia. rewrite right_id //.
@@ -2457,15 +2444,15 @@ Section heapGS.
   Qed.
 
   Lemma chunk_resize_spec_atomic Ψ l sz sz' n v' :
-    (0 ≤ n ≤ sz)%Z →
-    (0 ≤ n ≤ sz')%Z →
+    Z.to_nat n ≤ Z.to_nat sz →
+    Z.to_nat n ≤ Z.to_nat sz' →
     {{{
-      Ψ 0 [] ∗
+      ▷ Ψ 0 [] ∗
       □ (
         ∀ i vs,
         ⌜i < Z.to_nat n ∧ i = length vs⌝ -∗
         Ψ i vs -∗
-        chunk_au_load l i (λ v,
+        chunk_au_load l i (λ v, ▷
           Ψ (S i) (vs ++ [v])
         )
       )
@@ -2479,14 +2466,14 @@ Section heapGS.
       if decide (0 < sz')%Z then meta_token l' ⊤ else True
     }}}.
   Proof.
-    iIntros ((Hsz1 & Hsz2) (Hsz'1 & Hsz'2)) "%Φ (HΨ & #Hau) HΦ".
+    iIntros "%Hn1 %Hn2 %Φ (HΨ & #Hau) HΦ".
     wp_rec.
-    wp_smart_apply (chunk_make_spec with "[//]"); first lia. iIntros "%l' (Hmodel' & Hmeta)".
+    wp_smart_apply (chunk_make_spec with "[//]"). iIntros "%l' (Hmodel' & Hmeta)".
     pose Ψ' i vs o := (
       chunk_model l' (DfracOwn 1) (vs ++ replicate (Z.to_nat sz' - i) v') ∗
       from_option (λ v, Ψ (S i) (vs ++ [v])) (Ψ i vs) o
     )%I.
-    wp_smart_apply (chunk_copy_spec_atomic Ψ' with "[Hmodel' $HΨ]"); [done | | iSmash].
+    wp_smart_apply (chunk_copy_spec_atomic Ψ' with "[Hmodel' $HΨ]"); last iSmash.
     repeat iSplit.
     - rewrite Nat.sub_0_r. iSmash.
     - iIntros "!> %i %vs (%Hi1 & %Hi2) (Hmodel' & HΨ)".
@@ -2494,9 +2481,7 @@ Section heapGS.
       iSmash.
     - iIntros "!> %i %vs %v (%Hi1 & %Hi2) (Hmodel' & HΨ)".
       iDestruct (chunk_model_update i with "Hmodel'") as "(H↦ & Hmodel')".
-      { rewrite Hi2 lookup_app_r //. rewrite Nat.sub_diag lookup_replicate.
-        naive_solver lia.
-      }
+      { rewrite lookup_app_r; last lia. rewrite lookup_replicate. naive_solver lia. }
       iAuIntro. iAaccIntro with "H↦"; first iSmash. iIntros "H↦ !>". iFrame.
       iDestruct ("Hmodel'" with "H↦") as "Hmodel'".
       rewrite insert_app_r_alt; last lia. rewrite insert_replicate_lt; last lia.
@@ -2504,9 +2489,9 @@ Section heapGS.
       iSmash.
   Qed.
   Lemma chunk_resize_spec l dq vs (sz : Z) sz' n v' :
-    sz = length vs →
-    (n ≤ sz)%Z →
-    (0 ≤ n ≤ sz')%Z →
+    Z.to_nat sz = length vs →
+    Z.to_nat n ≤ Z.to_nat sz →
+    Z.to_nat n ≤ Z.to_nat sz' →
     {{{
       chunk_model l dq vs
     }}}
@@ -2518,7 +2503,7 @@ Section heapGS.
       if decide (0 < sz')%Z then meta_token l' ⊤ else True
     }}}.
   Proof.
-    iIntros (Hsz1 Hsz2 (Hsz'1 & Hsz'2)) "%Φ Hmodel HΦ".
+    iIntros "%Hsz %Hn1 %Hn2 %Φ Hmodel HΦ".
     pose Ψ i vs_done := (
       ⌜vs_done = take i vs⌝ ∗
       chunk_model l dq vs
@@ -2532,14 +2517,14 @@ Section heapGS.
   Qed.
 
   Lemma chunk_grow_spec_atomic Ψ l sz sz' v' :
-    (0 ≤ sz ≤ sz')%Z →
+    Z.to_nat sz ≤ Z.to_nat sz' →
     {{{
-      Ψ 0 [] ∗
+      ▷ Ψ 0 [] ∗
       □ (
         ∀ i vs,
         ⌜i < Z.to_nat sz ∧ i = length vs⌝ -∗
         Ψ i vs -∗
-        chunk_au_load l i (λ v,
+        chunk_au_load l i (λ v, ▷
           Ψ (S i) (vs ++ [v])
         )
       )
@@ -2553,13 +2538,13 @@ Section heapGS.
       if decide (0 < sz')%Z then meta_token l' ⊤ else True
     }}}.
   Proof.
-    iIntros ((Hsz & Hsz')) "%Φ (HΨ & #Hau) HΦ".
+    iIntros "%Hsz %Φ (HΨ & #Hau) HΦ".
     wp_rec.
     wp_smart_apply (chunk_resize_spec_atomic Ψ with "[$HΨ $Hau]"); [done.. | iSmash].
   Qed.
   Lemma chunk_grow_spec l dq vs (sz : Z) sz' v :
-    sz = length vs →
-    (sz ≤ sz')%Z →
+    Z.to_nat sz = length vs →
+    Z.to_nat sz ≤ Z.to_nat sz' →
     {{{
       chunk_model l dq vs
     }}}
@@ -2573,19 +2558,19 @@ Section heapGS.
   Proof.
     iIntros "%Hsz %Hsz' %Φ Hmodel HΦ".
     wp_rec.
-    wp_smart_apply (chunk_resize_spec with "Hmodel"); [lia.. |].
+    wp_smart_apply (chunk_resize_spec with "Hmodel"); [done.. |].
     iSteps. rewrite firstn_all2; last lia. iSmash.
   Qed.
 
   Lemma chunk_shrink_spec_atomic Ψ l sz sz' :
-    (0 ≤ sz' ≤ sz)%Z →
+    Z.to_nat sz' ≤ Z.to_nat sz →
     {{{
-      Ψ 0 [] ∗
+      ▷ Ψ 0 [] ∗
       □ (
         ∀ i vs,
         ⌜i < Z.to_nat sz' ∧ i = length vs⌝ -∗
         Ψ i vs -∗
-        chunk_au_load l i (λ v,
+        chunk_au_load l i (λ v, ▷
           Ψ (S i) (vs ++ [v])
         )
       )
@@ -2599,14 +2584,14 @@ Section heapGS.
       if decide (0 < sz')%Z then meta_token l' ⊤ else True
     }}}.
   Proof.
-    iIntros ((Hsz & Hsz')) "%Φ (HΨ & #Hau) HΦ".
+    iIntros "%Hsz %Φ (HΨ & #Hau) HΦ".
     wp_rec.
     wp_smart_apply (chunk_resize_spec_atomic Ψ with "[$HΨ $Hau]"); [done.. |].
     iSteps. rewrite Nat.sub_diag right_id. iSmash.
   Qed.
   Lemma chunk_shrink_spec l dq vs (sz : Z) sz' :
-    sz = length vs →
-    (0 ≤ sz' ≤ sz)%Z →
+    Z.to_nat sz = length vs →
+    Z.to_nat sz' ≤ Z.to_nat sz →
     {{{
       chunk_model l dq vs
     }}}
@@ -2620,19 +2605,18 @@ Section heapGS.
   Proof.
     iIntros "%Hsz %Hsz' %Φ Hmodel HΦ".
     wp_rec.
-    wp_smart_apply (chunk_resize_spec with "Hmodel"); [lia.. |].
+    wp_smart_apply (chunk_resize_spec with "Hmodel"); [done.. |].
     iSteps. rewrite Nat.sub_diag right_id. iSmash.
   Qed.
 
   Lemma chunk_clone_spec_atomic Ψ l sz :
-    (0 ≤ sz)%Z →
     {{{
-      Ψ 0 [] ∗
+      ▷ Ψ 0 [] ∗
       □ (
         ∀ i vs,
         ⌜i < Z.to_nat sz ∧ i = length vs⌝ -∗
         Ψ i vs -∗
-        chunk_au_load l i (λ v,
+        chunk_au_load l i (λ v, ▷
           Ψ (S i) (vs ++ [v])
         )
       )
@@ -2646,12 +2630,12 @@ Section heapGS.
       if decide (0 < sz)%Z then meta_token l' ⊤ else True
     }}}.
   Proof.
-    iIntros "%Hsz %Φ (HΨ & #Hau) HΦ".
+    iIntros "%Φ (HΨ & #Hau) HΦ".
     wp_rec.
     wp_smart_apply (chunk_shrink_spec_atomic Ψ with "[$HΨ $Hau]"); [done | iSmash].
   Qed.
   Lemma chunk_clone_spec l dq vs (sz : Z) :
-    sz = length vs →
+    Z.to_nat sz = length vs →
     {{{
       chunk_model l dq vs
     }}}
@@ -2667,7 +2651,516 @@ Section heapGS.
     wp_rec.
     wp_smart_apply (chunk_shrink_spec with "Hmodel"); [lia.. |]. iIntros "%l' (Hmodel & Hmodel' & Hmeta)".
     iApply "HΦ".
-    rewrite Hsz Nat2Z.id firstn_all. iSmash.
+    rewrite Hsz firstn_all. iSmash.
+  Qed.
+
+  Definition chunk_type τ `{!iType _ τ} (sz : nat) l : iProp Σ :=
+    inv nroot (
+      ∃ vs,
+      ⌜sz = length vs⌝ ∗
+      chunk_model l (DfracOwn 1) vs ∗ [∗ list] v ∈ vs, τ v
+    ).
+  #[global] Instance chunk_type_persistent τ `{!iType _ τ} sz l :
+    Persistent (chunk_type τ sz l).
+  Proof.
+    apply _.
+  Qed.
+
+  Lemma chunk_type_0 τ `{!iType _ τ} l :
+    ⊢ |={⊤}=>
+      chunk_type τ 0 l.
+  Proof.
+    iApply inv_alloc. iExists []. iSmash.
+  Qed.
+
+  Lemma chunk_type_shift (i : Z) τ `{!iType _ τ} (sz : nat) l :
+    (0 ≤ i < sz)%Z →
+    chunk_type τ sz l ⊢
+    chunk_type τ (sz - Z.to_nat i) (l +ₗ i).
+  Proof.
+    iIntros "%Hi #Hl".
+    Z_to_nat i. rewrite Nat2Z.id.
+    iApply (inv_alter with "Hl"). iIntros "!> !> (%vs & %Hvs & Hmodel & Hvs)".
+    rewrite -(take_drop i vs).
+    iDestruct (chunk_model_app_2 with "Hmodel") as "(Hmodel1 & Hmodel2)"; first done.
+    iDestruct (big_sepL_app with "Hvs") as "(Hvs1 & Hvs2)".
+    iSplitL "Hmodel2 Hvs2".
+    - iExists (drop i vs). iFrame.
+      rewrite take_length drop_length Nat.min_l; last lia. iSmash.
+    - iIntros "(%vs2 & %Hvs2 & Hmodel2 & Hvs2)".
+      iDestruct (chunk_model_app_1 with "Hmodel1 Hmodel2") as "Hmodel".
+      { rewrite take_length. lia. }
+      iExists (take i vs ++ vs2). iFrame.
+      rewrite app_length take_length Nat.min_l; last lia. iSmash.
+  Qed.
+
+  Lemma chunk_type_le sz' τ `{!iType _ τ} sz l :
+    (sz' ≤ sz) →
+    chunk_type τ sz l ⊢
+    chunk_type τ sz' l.
+  Proof.
+    iIntros "%Hsz #Hl".
+    iApply (inv_alter with "Hl"). iIntros "!> !> (%vs & %Hvs & Hmodel & Hvs)".
+    rewrite -(take_drop sz' vs).
+    iDestruct (chunk_model_app_2 with "Hmodel") as "(Hmodel1 & Hmodel2)"; first done.
+    iDestruct (big_sepL_app with "Hvs") as "(Hvs1 & Hvs2)".
+    iSplitL "Hmodel1 Hvs1".
+    - iExists (take sz' vs). iFrame.
+      rewrite take_length. iSmash.
+    - iIntros "(%vs1 & %Hvs1 & Hmodel1 & Hvs1)".
+      iDestruct (chunk_model_app_1 with "Hmodel1 Hmodel2") as "Hmodel".
+      { rewrite take_length. lia. }
+      iExists (vs1 ++ drop sz' vs). iFrame.
+      rewrite app_length drop_length. iSmash.
+  Qed.
+
+  Lemma chunk_make_type τ `{!iType _ τ} (sz : Z) v :
+    {{{
+      τ v
+    }}}
+      chunk_make #sz v
+    {{{ l,
+      RET #l;
+      chunk_type τ (Z.to_nat sz) l
+    }}}.
+  Proof.
+    iIntros "%Φ #Hv HΦ".
+    wp_rec. wp_pures.
+    case_bool_decide; wp_pures.
+    - wp_alloc l as "Hl"; first done.
+      iApply "HΦ".
+      iApply inv_alloc. iExists (replicate (Z.to_nat sz) v).
+      iSplit; first rewrite replicate_length //.
+      iSplitL; first rewrite /array //.
+      iApply big_sepL_intro. iIntros "!> %i %_v" ((-> & Hi)%lookup_replicate).
+      iSmash.
+    - iApply "HΦ".
+      iApply inv_alloc. iExists []. iSmash.
+  Qed.
+
+  Lemma chunk_get_type τ `{!iType _ τ} (sz : nat) l (i : Z) :
+    (0 ≤ i < sz)%Z →
+    {{{
+      chunk_type τ sz l
+    }}}
+      !#(l +ₗ i)
+    {{{ v,
+      RET v;
+      τ v
+    }}}.
+  Proof.
+    iIntros "%Hi %Φ #Hl HΦ".
+    Z_to_nat i.
+    iInv "Hl" as "(%vs & >%Hvs & Hmodel & #Hvs)".
+    feed pose proof (list_lookup_lookup_total_lt vs i); first lia.
+    iDestruct (chunk_model_lookup_acc with "Hmodel") as "(H↦ & Hmodel)"; first done.
+    wp_load.
+    iDestruct (big_sepL_lookup with "Hvs") as "Hv"; first done.
+    iSmash.
+  Qed.
+
+  Lemma chunk_set_type τ `{!iType _ τ} (sz : nat) l (i : Z) v :
+    (0 ≤ i < sz)%Z →
+    {{{
+      chunk_type τ sz l ∗
+      τ v
+    }}}
+      #(l +ₗ i) <- v
+    {{{
+      RET #(); True
+    }}}.
+  Proof.
+    iIntros "%Hi %Φ (#Hl & #Hv) HΦ".
+    Z_to_nat i.
+    iInv "Hl" as "(%vs & >%Hvs & Hmodel & Hvs)".
+    feed pose proof (list_lookup_lookup_total_lt vs i); first lia.
+    iDestruct (chunk_model_update with "Hmodel") as "(H↦ & Hmodel)"; first done.
+    wp_store.
+    iDestruct (big_sepL_insert_acc with "Hvs") as "(_ & Hvs)"; first done.
+    iModIntro. iSplitR "HΦ"; last iSmash. iExists (<[i := v]> vs).
+    iSteps. rewrite insert_length //.
+  Qed.
+
+  Lemma chunk_foldli_type τ `{!iType _ τ} υ `{!iType _ υ} l sz sz_ acc fn :
+    sz_ = Z.of_nat sz →
+    {{{
+      chunk_type τ sz l ∗
+      υ acc ∗
+      (υ --> nat_upto_type sz --> τ --> υ)%T fn
+    }}}
+      chunk_foldli #l #sz_ acc fn
+    {{{ acc',
+      RET acc';
+      υ acc'
+    }}}.
+  Proof.
+    iIntros (->) "%Φ (#Hl & Hacc & #Hfn) HΦ".
+    pose (Ψ i vs o acc := (
+      from_option τ True o ∗
+      υ acc
+    )%I).
+    wp_apply (chunk_foldli_spec_atomic Ψ with "[$Hacc]"); last iSmash.
+    clear acc. iSplit.
+    - iIntros "!> %i %vs_done %acc (%Hi1 & %Hi2) HΨ".
+      iAuIntro.
+      iInv "Hl" as "(%vs & >%Hvs & >Hmodel & #Hvs)".
+      feed pose proof (list_lookup_lookup_total_lt vs i); first lia.
+      iDestruct (chunk_model_lookup_acc with "Hmodel") as "(H↦ & Hmodel)"; first done.
+      iAaccIntro with "H↦"; first iSmash.
+      iDestruct (big_sepL_lookup with "Hvs") as "Hv"; first done.
+      iSmash.
+    - iIntros "!> %i %vs_done %v %acc (%Hi1 & %Hi2) (Hv & Hacc)".
+      wp_apply (wp_wand with "(Hfn Hacc)"). iClear "Hfn". clear fn. iIntros "%fn Hfn".
+      wp_apply (wp_wand with "(Hfn [])"); first iSmash. clear fn. iIntros "%fn Hfn".
+      wp_apply (wp_wand with "(Hfn Hv)").
+      iSmash.
+  Qed.
+
+  Lemma chunk_foldl_type τ `{!iType _ τ} υ `{!iType _ υ} l sz sz_ acc fn :
+    sz_ = Z.of_nat sz →
+    {{{
+      chunk_type τ sz l ∗
+      υ acc ∗
+      (υ --> τ --> υ)%T fn
+    }}}
+      chunk_foldl #l #sz_ acc fn
+    {{{ acc',
+      RET acc';
+      υ acc'
+    }}}.
+  Proof.
+    iIntros (->) "%Φ (#Hl & #Hacc & #Hfn) HΦ".
+    wp_rec.
+    wp_smart_apply (chunk_foldli_type τ υ with "[$Hl $Hacc]"); [done | iSmash..].
+  Qed.
+
+  Lemma chunk_foldri_type τ `{!iType _ τ} υ `{!iType _ υ} l sz sz_ acc fn :
+    sz_ = Z.of_nat sz →
+    {{{
+      chunk_type τ sz l ∗
+      υ acc ∗
+      (nat_upto_type sz --> τ --> υ --> υ)%T fn
+    }}}
+      chunk_foldri #l #sz_ fn acc
+    {{{ acc',
+      RET acc';
+      υ acc'
+    }}}.
+  Proof.
+    iIntros (->) "%Φ (#Hl & Hacc & #Hfn) HΦ".
+    pose (Ψ i acc o vs := (
+      from_option τ True o ∗
+      υ acc
+    )%I).
+    wp_apply (chunk_foldri_spec_atomic Ψ with "[$Hacc]"); last iSmash.
+    clear acc. repeat iSplit.
+    - iIntros "!> %i %acc %vs_done %Hi HΨ".
+      iAuIntro.
+      iInv "Hl" as "(%vs & >%Hvs & >Hmodel & #Hvs)".
+      feed pose proof (list_lookup_lookup_total_lt vs i); first lia.
+      iDestruct (chunk_model_lookup_acc with "Hmodel") as "(H↦ & Hmodel)"; first done.
+      iAaccIntro with "H↦"; first iSmash.
+      iDestruct (big_sepL_lookup with "Hvs") as "Hv"; first done.
+      iSmash.
+    - iIntros "!> %i %v %acc %vs_done %Hi (Hv & Hacc)".
+      wp_apply (wp_wand with "(Hfn [])"); first iSmash. iClear "Hfn". clear fn. iIntros "%fn Hfn".
+      wp_apply (wp_wand with "(Hfn Hv)"). clear fn. iIntros "%fn Hfn".
+      wp_apply (wp_wand with "(Hfn Hacc)").
+      iSmash.
+  Qed.
+
+  Lemma chunk_foldr_type τ `{!iType _ τ} υ `{!iType _ υ} l sz sz_ acc fn :
+    sz_ = Z.of_nat sz →
+    {{{
+      chunk_type τ sz l ∗
+      υ acc ∗
+      (τ --> υ --> υ)%T fn
+    }}}
+      chunk_foldr #l #sz_ fn acc
+    {{{ acc',
+      RET acc';
+      υ acc'
+    }}}.
+  Proof.
+    iIntros (->) "%Φ (#Hl & #Hacc & #Hfn) HΦ".
+    wp_rec.
+    wp_smart_apply (chunk_foldri_type τ υ with "[$Hl $Hacc]"); [done | iSmash..].
+  Qed.
+
+  Lemma chunk_iteri_type τ `{!iType _ τ} l sz sz_ fn :
+    sz_ = Z.of_nat sz →
+    {{{
+      chunk_type τ sz l ∗
+      (nat_upto_type sz --> τ --> unit_type)%T fn
+    }}}
+      chunk_iteri #l #sz_ fn
+    {{{
+      RET #(); True
+    }}}.
+  Proof.
+    iIntros (->) "%Φ (#Hl & #Hfn) HΦ".
+    wp_rec.
+    wp_smart_apply (chunk_foldli_type τ unit_type with "[$Hl]"); [done | iSmash..].
+  Qed.
+
+  Lemma chunk_iter_type τ `{!iType _ τ} l sz sz_ fn :
+    sz_ = Z.of_nat sz →
+    {{{
+      chunk_type τ sz l ∗
+      (τ --> unit_type)%T fn
+    }}}
+      chunk_iter #l #sz_ fn
+    {{{
+      RET #(); True
+    }}}.
+  Proof.
+    iIntros (->) "%Φ (#Hl & #Hfn) HΦ".
+    wp_rec.
+    wp_smart_apply (chunk_iteri_type τ with "[$Hl]"); [done | iSmash..].
+  Qed.
+
+  Lemma chunk_applyi_type τ `{!iType _ τ} l sz sz_ fn :
+    sz_ = Z.of_nat sz →
+    {{{
+      chunk_type τ sz l ∗
+      (nat_upto_type sz --> τ --> τ)%T fn
+    }}}
+      chunk_applyi #l #sz_ fn
+    {{{
+      RET #(); True
+    }}}.
+  Proof.
+    iIntros (->) "%Φ (#Hl & #Hfn) HΦ".
+    wp_rec.
+    wp_smart_apply (chunk_iteri_type τ with "[$Hl]"); [done | | iSmash].
+    iIntros "!> % (%i & -> & %Hi)". wp_pures. iIntros "!> !> %v Hv".
+    wp_smart_apply (wp_wand with "(Hfn [])"); first iSmash. iClear "Hfn". clear fn. iIntros "%fn Hfn".
+    wp_apply (wp_wand with "(Hfn Hv)"). iIntros "%w Hw".
+    wp_smart_apply (chunk_set_type with "[$Hl $Hw]"); first lia.
+    iSmash.
+  Qed.
+
+  Lemma chunk_apply_type τ `{!iType _ τ} l sz sz_ fn :
+    sz_ = Z.of_nat sz →
+    {{{
+      chunk_type τ sz l ∗
+      (τ --> τ)%T fn
+    }}}
+      chunk_apply #l #sz_ fn
+    {{{
+      RET #(); True
+    }}}.
+  Proof.
+    iIntros (->) "%Φ (#Hl & #Hfn) HΦ".
+    wp_rec.
+    wp_smart_apply (chunk_applyi_type τ with "[$Hl]"); [done | iSmash..].
+  Qed.
+
+  Lemma chunk_initi_type τ `{!iType _ τ} (sz : Z) fn :
+    {{{
+      (nat_upto_type (Z.to_nat sz) --> τ)%T fn
+    }}}
+      chunk_initi #sz fn
+    {{{ l,
+      RET #l;
+      chunk_type τ (Z.to_nat sz) l
+    }}}.
+  Proof.
+    iIntros "%Φ #Hfn HΦ".
+    wp_rec.
+    wp_smart_apply (chunk_make_spec with "[//]"). iIntros "%l (Hmodel & _)".
+    wp_smart_apply (chunk_applyi_spec_disentangled (λ _, τ) with "[$Hmodel]").
+    { rewrite replicate_length. lia. }
+    { iIntros "!> %i %v %Hlookup".
+      wp_smart_apply (wp_wand with "(Hfn [])"); last iSmash.
+      apply lookup_lt_Some in Hlookup. rewrite replicate_length in Hlookup. iSmash.
+    }
+    iIntros "%vs (%Hvs & Hmodel & Hvs)". rewrite replicate_length in Hvs.
+    iSmash.
+  Qed.
+
+  Lemma chunk_init_type τ `{!iType _ τ} (sz : Z) fn :
+    {{{
+      (unit_type --> τ)%T fn
+    }}}
+      chunk_init #sz fn
+    {{{ l,
+      RET #l;
+      chunk_type τ (Z.to_nat sz) l
+    }}}.
+  Proof.
+    iIntros "%Φ #Hfn HΦ".
+    wp_rec.
+    wp_smart_apply (chunk_initi_type τ with "[] HΦ").
+    iSmash.
+  Qed.
+
+  Lemma chunk_mapi_type τ `{!iType _ τ} υ `{!iType _ υ} l sz sz_ fn :
+    sz_ = Z.of_nat sz →
+    {{{
+      chunk_type τ sz l ∗
+      (nat_upto_type sz --> τ --> υ)%T fn
+    }}}
+      chunk_mapi #l #sz_ fn
+    {{{ l',
+      RET #l';
+      chunk_type υ sz l'
+    }}}.
+  Proof.
+    iIntros (->) "%Φ (#Hl & #Hfn) HΦ".
+    wp_rec.
+    wp_smart_apply (chunk_initi_type υ).
+    { iIntros "!> % (%i & -> & %Hi)".
+      wp_smart_apply (chunk_get_type with "Hl"); first lia.
+      iSmash.
+    }
+    rewrite Nat2Z.id. iSmash.
+  Qed.
+
+  Lemma chunk_map_type τ `{!iType _ τ} υ `{!iType _ υ} l sz sz_ fn :
+    sz_ = Z.of_nat sz →
+    {{{
+      chunk_type τ sz l ∗
+      (τ --> υ)%T fn
+    }}}
+      chunk_map #l #sz_ fn
+    {{{ l',
+      RET #l';
+      chunk_type υ sz l'
+    }}}.
+  Proof.
+    iIntros (->) "%Φ (#Hl & #Hfn) HΦ".
+    wp_rec.
+    wp_smart_apply (chunk_mapi_type τ υ with "[] HΦ"); first done.
+    iFrame "#∗". iSmash.
+  Qed.
+
+  Lemma chunk_copy_type τ `{!iType _ τ} l1 sz1 sz1_ l2 sz2 :
+    sz1_ = Z.of_nat sz1 →
+    sz1 ≤ sz2 →
+    {{{
+      chunk_type τ sz1 l1 ∗
+      chunk_type τ sz2 l2
+    }}}
+      chunk_copy #l1 #sz1_ #l2
+    {{{
+      RET #(); True
+    }}}.
+  Proof.
+    iIntros (->) "%Hsz %Φ (#Hl1 & #Hl2) HΦ".
+    wp_rec.
+    wp_smart_apply (chunk_iteri_type τ with "[] HΦ"); first done.
+    iFrame "#∗". iIntros "!> % (%i & -> & %Hi)". wp_pures. iIntros "!> !> %v Hv".
+    wp_smart_apply (chunk_set_type with "[$Hl2 $Hv]"); first lia.
+    iSmash.
+  Qed.
+
+  Lemma chunk_resize_type τ `{!iType _ τ} l sz sz_ sz' n v' :
+    sz_ = Z.of_nat sz →
+    (n ≤ sz)%Z →
+    (n ≤ sz')%Z →
+    {{{
+      chunk_type τ sz l ∗
+      if decide (n < sz')%Z then τ v' else True
+    }}}
+      chunk_resize #l #sz_ #sz' #n v'
+    {{{ l',
+      RET #l';
+      chunk_type τ (Z.to_nat sz') l'
+    }}}.
+  Proof.
+    iIntros (->) "%Hn1 %Hn2 %Φ (#Hl & Hv') HΦ".
+    wp_rec.
+    wp_smart_apply (chunk_make_spec with "[//]"). iIntros "%l' (Hmodel' & _)".
+    pose (Ψ i vs' o := (
+      chunk_model l' (DfracOwn 1) (vs' ++ replicate (Z.to_nat sz' - i) v') ∗
+      ([∗ list] v' ∈ vs', τ v') ∗
+      from_option τ True o
+    )%I).
+    wp_smart_apply (chunk_copy_spec_atomic Ψ with "[Hmodel']"); last first.
+    { iIntros "%vs' (%Hvs' & (Hmodel' & Hvs' & _))".
+      wp_pures.
+      iApply "HΦ".
+      iApply inv_alloc. iExists _. iFrame "Hmodel'".
+      iSplit. { rewrite app_length replicate_length. iSmash. }
+      iSplit; first iSmash.
+      iApply big_sepL_replicate_2.
+      case_decide.
+      - iDestruct "Hv'" as "#Hv'".
+        iApply big_sepL_intro. auto.
+      - assert (n = sz') as -> by lia. rewrite Nat.sub_diag //.
+    }
+    iSplit; last iSplit.
+    - iSteps. rewrite Nat.sub_0_r. iSmash.
+    - iIntros "!> %i %vs' (%Hi1 & %Hi2) (Hmodel' & Hvs' & _)".
+      iAuIntro.
+      iInv "Hl" as "(%vs & >%Hvs & >Hmodel & #Hvs)".
+      feed pose proof (list_lookup_lookup_total_lt vs i); first lia.
+      iDestruct (chunk_model_lookup_acc with "Hmodel") as "(H↦ & Hmodel)"; first done.
+      iDestruct (big_sepL_lookup with "Hvs") as "Hv"; first done.
+      iAaccIntro with "H↦"; iSmash.
+    - iIntros "!> %i %vs' %v'' (%Hi1 & %Hi2) (Hmodel' & Hvs' & Hv'')".
+      iDestruct (chunk_model_update i with "Hmodel'") as "(H↦' & Hmodel')".
+      { rewrite lookup_app_r; last lia. rewrite lookup_replicate. naive_solver lia. }
+      iAuIntro. iAaccIntro with "H↦'"; first iSmash. iIntros "H↦' !> !>". iFrame. rewrite /= right_id.
+      iDestruct ("Hmodel'" with "H↦'") as "Hmodel'".
+      rewrite insert_app_r_alt; last lia. rewrite insert_replicate_lt; last lia.
+      rewrite Hi2 Nat.sub_diag /= Nat.sub_1_r -Nat.sub_succ_r -(assoc (++)).
+      iSmash.
+  Qed.
+
+  Lemma chunk_grow_type τ `{!iType _ τ} l sz sz_ sz' v' :
+    sz_ = Z.of_nat sz →
+    (sz ≤ sz')%Z →
+    {{{
+      chunk_type τ sz l ∗
+      τ v'
+    }}}
+      chunk_grow #l #sz_ #sz' v'
+    {{{ l',
+      RET #l';
+      chunk_type τ (Z.to_nat sz') l'
+    }}}.
+  Proof.
+    iIntros (->) "%Hsz %Φ (#Hl & #Hv') HΦ".
+    wp_rec.
+    wp_smart_apply (chunk_resize_type with "[$Hl] HΦ"); [done.. |].
+    case_decide; iSmash.
+  Qed.
+
+  Lemma chunk_shrink_type τ `{!iType _ τ} l sz sz_ sz' :
+    sz_ = Z.of_nat sz →
+    (sz' ≤ sz)%Z →
+    {{{
+      chunk_type τ sz l
+    }}}
+      chunk_shrink #l #sz_ #sz'
+    {{{ l',
+      RET #l';
+      chunk_type τ (Z.to_nat sz') l'
+    }}}.
+  Proof.
+    iIntros (->) "%Hsz %Φ #Hl HΦ".
+    wp_rec.
+    wp_smart_apply (chunk_resize_type with "[$Hl] HΦ"); [done.. |].
+    rewrite decide_False //. lia.
+  Qed.
+
+  Lemma chunk_clone_type τ `{!iType _ τ} l sz sz_ :
+    sz_ = Z.of_nat sz →
+    {{{
+      chunk_type τ sz l
+    }}}
+      chunk_clone #l #sz_
+    {{{ l',
+      RET #l';
+      chunk_type τ sz l'
+    }}}.
+  Proof.
+    iIntros (->) "%Φ #Hl HΦ".
+    wp_rec.
+    wp_smart_apply (chunk_shrink_type with "Hl"); [done.. |].
+    rewrite Nat2Z.id. iSmash.
   Qed.
 End heapGS.
 
